Fix definition of `PCR.Congruent`

Eqsat/EGraph.lean
@@ -1,6 +1,7 @@
 import Eqsat.TreeAutomaton
 import Eqsat.PCR
 
+/-- Definition 3 -/
 structure EGraph (S Q) [Signature S] extends auto : TreeAutomaton S Q where
   det      : auto.Deterministic
   reach    : auto.Reachable
@@ -17,6 +18,7 @@ abbrev ENode (_ : EGraph S Q) := TreeAutomaton.Transition S Q
 abbrev EClass.Represents (c : EClass graph) (t : Term S) : Prop :=
   graph.Accepts c t
 
+/-- Definition 5 -/
 def pcr (graph : EGraph S Q) : PCR S where
   rel t₁ t₂ :=
     ∃ c : EClass graph, c.Represents t₁ ∧ c.Represents t₂
@@ -29,8 +31,62 @@ def pcr (graph : EGraph S Q) : PCR S where
     have := graph.det h₁ h₂
     simp_all
   congr h mem := by
+    rename_i fn as bs
     simp_all [PER.support]
+    obtain ⟨c, hc⟩ := mem
+    refine ⟨c, hc, ?_⟩
+    have ⟨qs, hq₁, hq₂⟩ := hc.final
+    apply Relation.ReflTransGen.tail ?_ (TreeAutomaton.step_of_transition hq₁)
+    · refine TRS.Steps.children (fun i => ?_)
+      have ⟨_, hc₁, hc₂⟩ := h i
+      obtain ⟨rfl⟩ := graph.det hc₁ <| TreeAutomaton.steps_child hq₂ i
+      exact hc₂
   reach h i := by
     simp only [PER.support, and_self, Set.mem_setOf_eq] at *
     obtain ⟨_, h⟩ := h
     apply h.child
+
+end EGraph
+
+/- Theorem 6 -/
+namespace PCR
+
+variable [Signature S] {graph : EGraph S Q}
+
+def egraph (pcr : PCR S) : EGraph S pcr.classes where
+  trans :=
+    { ⟨fn, qs, dst⟩ |
+      ∃ (as : Term.Args fn) (mem₁ : fn ° as ∈ pcr.support) (mem₂ : ∀ i, as i ∈ pcr.support),
+      dst = Quotient.mk' ⟨fn ° as, mem₁⟩ ∧
+      qs = fun i => Quotient.mk' ⟨as i, mem₂ i⟩
+    }
+  final    := ∅
+  no_final := rfl
+  det      := sorry
+  reach    := sorry
+
+theorem egraph_correct (pcr : PCR S) : pcr.egraph.pcr = pcr := by
+  ext t₁ t₂
+  induction t₁ generalizing t₂ <;> cases t₂ <;> try contradiction
+  case app.app fn₁ as₁ ih fn₂ as₂ =>
+    simp only [egraph, EGraph.pcr] at ih ⊢
+    apply Iff.intro (fun h => ?mp) (fun h => ?mpr)
+    case mp =>
+      obtain ⟨c, hc₁, hc₂⟩ := h
+      if hf : fn₁ = fn₂ then
+        subst hf
+        apply pcr.congr fun i => ih i (as₂ i) |>.mp ?_
+        -- TODO: There should be a lemma stating that (∃ c, Represents c t) coincides with
+        --       membership in the PCR's support.
+        · sorry
+        · sorry
+      else
+        sorry
+    case mpr h => sorry
+
+theorem egraph_unique {pcr : PCR S} (h : pcr = graph.pcr) : graph ≍ pcr.egraph := by
+  sorry
+  -- TODO: We might not be able to prove this up to HEq, but only some weaker notion of
+  --       isomorphism.
+
+end PCR
