Eqsat/PCR.lean
@@ -1,6 +1,7 @@
 import Eqsat.Term
 import Mathlib.Order.Defs.Unbundled
 
+@[ext]
 structure PER (α : Type _) where
   rel   : α → α → Prop
   symm  : Symmetric rel
@@ -14,16 +15,25 @@ namespace PER
 def support (per : PER α) : Set α :=
   { a | per a a }
 
+instance supportSetoid (per : PER α) : Setoid (support per) where
+  r a₁ a₂ := per.rel a₁ a₂
+  iseqv   := by grind [Equivalence, support, PER.symm, PER.trans, Symmetric, Transitive]
+
 variable [Signature S]
 
 def Congruent (per : PER <| Term S) : Prop :=
-  ∀ {fn : S} {as bs : Term.Args fn}, as = bs → fn ° as ∈ per.support → per (fn ° as) (fn ° bs)
+  ∀ {fn : S} {as bs : Term.Args fn},
+    (∀ i, per (as i) (bs i)) → fn ° as ∈ per.support → per (fn ° as) (fn ° bs)
 
 def Reachable (per : PER <| Term S) : Prop :=
   ∀ {fn : S} {as : Term.Args fn}, fn ° as ∈ per.support → ∀ i, as i ∈ per.support
 
 end PER
 
+@[ext]
 structure PCR (S) [Signature S] extends per : PER (Term S) where
   congr : per.Congruent
   reach : per.Reachable
+
+def PCR.classes [Signature S] (pcr : PCR S) : Type :=
+  Quotient <| PER.supportSetoid pcr.per
